%\documentclass{report}

\begin{document}
    \section{Groups}
    
    The first thing we would encounter in abstract algebra is a group... but you already encountered it. Refer to the chapter "Algebraic Structures" for the definition of a group and an Abelian group.
    
    If the context is obvious, we will skip $\cdot$ and write $ab$ instead of $a \cdot b$. The identity of $G$ will be denoted $e$ or $1$.
    
    \begin{thm} \label{thm_group_basics}
        If $G$ is a group, and $a,b,c \in G$, then \begin{enumerate}
            \item the identity of $G$ is unique.
            \item the inverse $a^{-1}$ is unique.
            \item $(a^{-1})^{-1}=a$.
            \item $(ab)^{-1} = b^{-1}a^{-1}$.
            \item if $ab=ac$, then $b=c$. Also, if $ba=ca$, then $b=c$.
        \end{enumerate}
    \end{thm}
    
    \begin{proof}
        \begin{enumerate} \item[]
        \item Let $e_1$ and $e_2$ be the identities of $G$. Then $e_1e_2=e_2e_1=e_1$, and $e_2e_1=e_1e_2=e_2$, from the definition of the identity. Therefore $e_1=e_2$.
        \item Let $b_1$ and $b_2$ the inverses of $a$. Then $b_1 = b_1(ab_2) = (b_1a)b_2 = b_2$.
        \item The definition of an inverse shows that $a$ is an inverse of $a^{-1}$. From (ii), such an inverse is unique.
        \item $(ab)b^{-1}a^{-1} = a(bb^{-1})a^{-1} = aa^{-1} = e$. Similarly $b^{-1}a^{-1}(ab) = e$. From (ii), the inverse of $ab$ is unique.
        \item $ab=ac \implies a^{-1}ab=a^{-1}ac \implies b=c$. Similar argument for $ba=ca$.
        \end{enumerate}
    \end{proof}

\end{document}